examples/Online_with_authn/DY.OnlineA.Invariants.fst
@@ -3,7 +3,6 @@ module DY.OnlineA.Invariants
 open Comparse 
 open DY.Core
 open DY.Lib
-
 open DY.Extend
 
 open DY.OnlineA.Data
@@ -34,21 +33,18 @@ open DY.OnlineA.Protocol
 %splice [ps_ack_t_is_well_formed] (gen_is_well_formed_lemma (`ack_t))
 %splice [ps_message_t_is_well_formed] (gen_is_well_formed_lemma (`message_t))
 
-instance crypto_usages_p : crypto_usages = default_crypto_usages
+instance crypto_usages_online : crypto_usages = default_crypto_usages
 
-#push-options "--ifuel 2"
-let crypto_p : crypto_predicates = { 
+#push-options "--ifuel 3"
+let crypto_predicates_online : crypto_predicates = { 
   default_crypto_predicates with 
   pke_pred = { 
     pred = (fun tr sk_usage pk msg ->
-    exists prin.
-    (
+    exists prin. (
       sk_usage == long_term_key_type_to_usage (LongTermPkeKey key_tag) prin /\
       (match parse message_t msg with
-      | Some (Ping ping) ->
+      | Some (Ping {alice; n_a}) ->
           let bob = prin in
-          let alice = ping.alice in
-          let n_a = ping.n_a in
           get_label tr n_a == nonce_label alice bob
 
           (* We add, that the Alice specified in the Ping message,
@@ -59,7 +55,7 @@ let crypto_p : crypto_predicates = {
              * the nonce n_a in the Ping
           *)
           /\ event_triggered tr alice (Initiating {alice; bob; n_a})
-      | Some (Ack ack) ->
+      | Some (Ack {n_a}) ->
           (* For nonce secrecy,
              we didn't have any conditions/guarantees in the Ack case.
              Now, we add that 
@@ -69,7 +65,7 @@ let crypto_p : crypto_predicates = {
              * the nonce (n_a) in the Ack
           *)
           let alice = prin in
-          exists bob. event_triggered tr bob (Responding {alice; bob; n_a = ack.n_a})
+          exists bob. event_triggered tr bob (Responding {alice; bob; n_a})
       | _ -> False
       ))
       ); 
@@ -82,9 +78,9 @@ let crypto_p : crypto_predicates = {
 
 /// Collecting the usages and prediates in the final crypto invariants
 
-instance crypto_invariants_p: crypto_invariants = {
-  usages = crypto_usages_p;
-  preds =  crypto_p
+instance crypto_invariants_online: crypto_invariants = {
+  usages = crypto_usages_online;
+  preds =  crypto_predicates_online
 }
 
 
@@ -96,13 +92,11 @@ instance crypto_invariants_p: crypto_invariants = {
 %splice [ps_state_t_is_well_formed] (gen_is_well_formed_lemma (`state_t))
 
 #push-options "--ifuel 2 --z3cliopt 'smt.qi.eager_threshold=50'"
-let state_predicate_p: local_state_predicate state_t = {
+let state_predicate_online: local_state_predicate state_t = {
   pred = (fun tr prin sess_id st ->
     match st with
-    | SentPing ping -> (
+    | SentPing {bob; n_a} -> (
         let alice = prin in
-        let bob = ping.bob in
-        let n_a = ping.n_a in
         is_secret (nonce_label alice bob) tr n_a
         (* We add, that the storing principal (alice),
            must have triggered an Initiating event with:
@@ -110,12 +104,10 @@ let state_predicate_p: local_state_predicate state_t = {
            * the bob stored in the state and
            * the nonce stored in the state
         *)
-        /\ event_triggered tr alice (Initiating {alice = alice; bob = bob; n_a = n_a})
+        /\ event_triggered tr alice (Initiating {alice; bob; n_a})
     )
-    | SentAck ack -> (
+    | SentAck {alice; n_a} -> (
         let bob = prin in
-        let alice = ack.alice in
-        let n_a = ack.n_a in
         is_knowable_by (principal_label bob) tr n_a
         (* Additionally, we enforce that
            the storing principal (bob) 
@@ -126,10 +118,8 @@ let state_predicate_p: local_state_predicate state_t = {
         *)
         /\ event_triggered tr bob (Responding {alice; bob; n_a})
     )
-    | ReceivedAck rack  -> (
+    | ReceivedAck {bob; n_a}  -> (
         let alice = prin in
-        let bob = rack.bob in
-        let n_a = rack.n_a in
         is_secret (nonce_label alice bob) tr n_a
 
         (* We add, that the storing principal (alice),
@@ -147,22 +137,19 @@ let state_predicate_p: local_state_predicate state_t = {
 #pop-options
 
 
-(*** Event Pred ***)
+(*** Event Predicates ***)
 
 /// As for messages and states,
-/// we also have prediates on events.
+/// we also have predicates on events.
 /// The intuition is similar:
 /// They say when an event is allowed to be triggered, or
 /// what guarantees we obtain, if we observe a specific event on the trace.
 
-let event_predicate_event_t: event_predicate event_t =
+let event_predicate_online: event_predicate event_t =
   fun tr prin e ->
   // prin is the principal triggering the event
     match e with    
-    | Initiating init -> (
-        let alice = init.alice in
-        let bob = init.bob in
-        let n_a = init.n_a in
+    | Initiating {alice; bob; n_a} -> (
         (* We may trigger the Initiating event only if,
            * the triggering principal is the first principal stored in the event (alice)
            * the nonce (n_a) in the event is labelled for 
@@ -175,10 +162,7 @@ let event_predicate_event_t: event_predicate event_t =
         is_secret (nonce_label alice bob) tr n_a /\
         rand_just_generated tr n_a
     )
-    | Responding resp -> (
-        let alice = resp.alice in
-        let bob = resp.bob in
-        let n_a = resp.n_a in
+    | Responding {alice; bob; n_a} -> (
         (* A Responding event may only be triggered if,
            * the triggering principal is the second principal stored in the event (bob)
            * if the stored nonce n_a has not leaked,
@@ -186,21 +170,15 @@ let event_predicate_event_t: event_predicate event_t =
              must have triggered an Initiating event with the same data
              as the Responding event
         *)
-        prin == bob
-        /\ (is_publishable tr n_a
-          \/ event_triggered tr alice (Initiating {alice; bob; n_a})
-        )
+        prin == bob /\ 
+        ( is_publishable tr n_a \/
+          event_triggered tr alice (Initiating {alice; bob; n_a}))
     )
-    | Finishing fin -> (
-        let alice = fin.alice in
-        let bob = fin.bob in
-        let n_a = fin.n_a in
-
+    | Finishing {alice; bob; n_a} -> (
         prin == alice /\
         event_triggered tr alice (Initiating {alice; bob; n_a}) /\
         ( is_corrupt tr (nonce_label alice bob) \/
-          event_triggered tr bob (Responding {alice; bob; n_a})
-        )
+          event_triggered tr bob (Responding {alice; bob; n_a}))
     )
 
 
@@ -209,13 +187,13 @@ let event_predicate_event_t: event_predicate event_t =
 let all_sessions = [
   pki_tag_and_invariant;
   private_keys_tag_and_invariant;
-  (|local_state_state.tag, local_state_predicate_to_local_bytes_state_predicate state_predicate_p|);
+  (|local_state_state.tag, local_state_predicate_to_local_bytes_state_predicate state_predicate_online|);
 ]
 
 /// Now we have an event type
-let all_events = [(event_event_t.tag, compile_event_pred event_predicate_event_t)]
+let all_events = [(event_event_t.tag, compile_event_pred event_predicate_online)]
 
-let trace_invariants_p: trace_invariants = {
+let trace_invariants_online: trace_invariants = {
   state_pred = mk_state_pred all_sessions;
   event_pred = mk_event_pred all_events;
 }
@@ -223,13 +201,12 @@ let trace_invariants_p: trace_invariants = {
 
 (*** Protocol Invariants ***)
 
-instance protocol_invariants_p: protocol_invariants = {
-  crypto_invs = crypto_invariants_p;
-  trace_invs = trace_invariants_p;
+instance protocol_invariants_online: protocol_invariants = {
+  crypto_invs = crypto_invariants_online;
+  trace_invs = trace_invariants_online;
 }
 
-
-(*** Helper Lemmas for the Secrecy Proof ***)
+/// Lemmas that the global state predicate contains all the local ones
 
 val all_sessions_has_all_sessions: unit -> Lemma (norm [delta_only [`%all_sessions; `%for_allP]; iota; zeta] (for_allP (has_local_bytes_state_predicate) all_sessions))
 let all_sessions_has_all_sessions () =
@@ -237,25 +214,24 @@ let all_sessions_has_all_sessions () =
   mk_state_pred_correct all_sessions;
   norm_spec [delta_only [`%all_sessions; `%for_allP]; iota; zeta] (for_allP (has_local_bytes_state_predicate) all_sessions)
 
-val protocol_invariants_p_has_p_session_invariant: squash (has_local_state_predicate state_predicate_p)
+val protocol_invariants_p_has_p_session_invariant: squash (has_local_state_predicate state_predicate_online)
 let protocol_invariants_p_has_p_session_invariant = all_sessions_has_all_sessions ()
 
-val protocol_invariants_p_has_pki_invariant: squash (has_pki_invariant #protocol_invariants_p)
+val protocol_invariants_p_has_pki_invariant: squash (has_pki_invariant #protocol_invariants_online)
 let protocol_invariants_p_has_pki_invariant = all_sessions_has_all_sessions ()
 
-val protocol_invariants_p_has_private_keys_invariant: squash (has_private_keys_invariant #protocol_invariants_p)
+val protocol_invariants_p_has_private_keys_invariant: squash (has_private_keys_invariant #protocol_invariants_online)
 let protocol_invariants_p_has_private_keys_invariant = all_sessions_has_all_sessions ()
 
+/// Lemmas that the global event predicate contains all the local ones
 
-/// We need similar lemmas for our event type
-
-val all_events_has_all_events: unit -> Lemma (norm [delta_only [`%all_events; `%for_allP]; iota; zeta] (for_allP (has_compiled_event_pred #protocol_invariants_p) all_events))
+val all_events_has_all_events: unit -> Lemma (norm [delta_only [`%all_events; `%for_allP]; iota; zeta] (for_allP (has_compiled_event_pred #protocol_invariants_online) all_events))
 let all_events_has_all_events () =
   assert_norm(List.Tot.no_repeats_p (List.Tot.map fst (all_events)));
-  mk_event_pred_correct #protocol_invariants_p all_events;
-  norm_spec [delta_only [`%all_events; `%for_allP]; iota; zeta] (for_allP (has_compiled_event_pred #protocol_invariants_p) all_events);
+  mk_event_pred_correct #protocol_invariants_online all_events;
+  norm_spec [delta_only [`%all_events; `%for_allP]; iota; zeta] (for_allP (has_compiled_event_pred #protocol_invariants_online) all_events);
   let dumb_lemma (x:prop) (y:prop): Lemma (requires x /\ x == y) (ensures y) = () in
-  dumb_lemma (for_allP (has_compiled_event_pred #protocol_invariants_p) all_events) (norm [delta_only [`%all_events; `%for_allP]; iota; zeta] (for_allP (has_compiled_event_pred #protocol_invariants_p) all_events))
+  dumb_lemma (for_allP (has_compiled_event_pred #protocol_invariants_online) all_events) (norm [delta_only [`%all_events; `%for_allP]; iota; zeta] (for_allP (has_compiled_event_pred #protocol_invariants_online) all_events))
 
-val protocol_invariants_p_has_event_t_invariant: squash (has_event_pred event_predicate_event_t)
+val protocol_invariants_p_has_event_t_invariant: squash (has_event_pred event_predicate_online)
 let protocol_invariants_p_has_event_t_invariant = all_events_has_all_events ()
